lib_bitmap/Bitmap5.fst
@@ -115,8 +115,8 @@ let bm_set_aux
 
 #push-options "--z3rlimit 50"
 let bm_set
-  (#n: nat)
-  (arr: array U64.t{A.length arr = n})
+  (#n: G.erased nat)
+  (arr: array U64.t{A.length arr = G.reveal n})
   (k: U32.t{U32.v k < U64.n * n})
   : Steel unit
   (A.varray arr)
